improve generic field library

src/Field.v
@@ -1,6 +1,27 @@
 Require Import Coq.setoid_ring.Cring.
 Generalizable All Variables.
 
+
+(*TODO: move *)
+Lemma Z_pos_pred_0 p : Z.pos p - 1 = 0 -> p=1%positive.
+Proof. destruct p; simpl in *; try discriminate; auto. Qed.
+
+Lemma Z_neg_succ_neg : forall a b, (Z.neg a + 1)%Z = Z.neg b -> a = Pos.succ b.
+Admitted.
+
+Lemma Z_pos_pred_pos : forall a b, (Z.pos a - 1)%Z = Z.pos b -> a = Pos.succ b.
+Admitted.
+
+Lemma Z_pred_neg p : (Z.neg p - 1)%Z = Z.neg (Pos.succ p).
+Admitted.
+
+(* teach nsatz to deal with the definition of power we are use *)
+Instance  reify_pow_pos (R:Type) `{Ring R}
+e1 lvar t1 n
+`{Ring (T:=R)}
+{_:reify e1 lvar t1}
+: reify (PEpow e1 (N.pos n)) lvar (pow_pos t1 n)|1.
+
 Class Field_ops (F:Type)
       `{Ring_ops F}
       {inv:F->F} := {}.
@@ -12,7 +33,7 @@ Notation "n / d" := (division n d).
 
 Module F.
 
-  Definition div `{Field_ops F} n d := mul n (inv d).
+  Definition div `{Field_ops F} n d := n * (inv d).
   Global Instance div_notation `{Field_ops F} : @Division F F := div.
 
   Class Field {F inv} `{FieldCring:Cring (R:=F)} {Fo:Field_ops F (inv:=inv)} :=
@@ -33,6 +54,8 @@ Module F.
 
   Section FieldProofs.
     Context `{Field F}.
+  
+    Definition unfold_div (x y:F) : x/y = x * inv y := eq_refl.
 
     Global Instance Proper_div :
       Proper (_==_ ==> _==_ ==> _==_) div.
@@ -41,6 +64,21 @@ Module F.
       repeat match goal with
              | [H: _ == _ |- _ ] => rewrite H; clear H
              end; reflexivity.
+    Qed.
+
+    Global Instance Proper_pow_pos : Proper (_==_==>eq==>_==_) pow_pos.
+    Proof.
+      cut (forall n (y x : F), x == y -> pow_pos x n == pow_pos y n);
+        [repeat intro; subst; eauto|].
+      induction n; simpl; intros; trivial;
+        repeat eapply ring_mult_comp; eauto.
+    Qed.
+      
+    Global Instance Propper_powZ : Proper (_==_==>eq==>_==_) powZ.
+    Proof.
+      repeat intro; subst; unfold powZ.
+      match goal with |- context[match ?x with _ => _ end] => destruct x end;
+        repeat (eapply Proper_pow_pos || f_equiv; trivial).
     Qed.
 
     Require Import Coq.setoid_ring.Field_theory Coq.setoid_ring.Field_tac.
@@ -53,9 +91,12 @@ Module F.
     Lemma power_theory_for_tactic : power_theory 1 _*_ _==_ NtoZ power.
     Proof. constructor; destruct n; reflexivity. Qed.
 
+    Create HintDb field_nonzero discriminated.
+    Hint Resolve field_one_neq_zero : field_nonzero.
+    Ltac field_nonzero := repeat split; auto 3 with field_nonzero.
     Ltac field_power_isconst t := Ncst t.
     Add Field FieldProofsAddField : field_theory_for_tactic
-                                      (postprocess [trivial],
+                                      (postprocess [field_nonzero],
                                        power_tac power_theory_for_tactic [field_power_isconst]).
 
     Lemma div_mul_idemp_l : forall a b, (a==0 -> False) -> a*b/a == b.
@@ -75,40 +116,138 @@ Module F.
       constructor; intros; eauto using mul_zero_why, field_one_neq_zero.
     Qed.
 
-    Lemma mul_inv_l : forall x, not (x == 0) -> inv x * x == 1.
-    Proof. intros. field. Qed.
+    Create HintDb field discriminated.
+    Hint Extern 5 (_ == _) => field_simplify_eq; nsatz : field.
+    Hint Extern 5 (_ <-> _) => split.
 
-    Lemma mul_inv_r : forall x, not (x == 0) -> x * inv x == 1.
-    Proof. intros. field. Qed.
+    Lemma mul_inv_l : forall x, not (x == 0) -> inv x * x == 1. Proof. auto with field. Qed.
+
+    Lemma mul_inv_r : forall x, not (x == 0) -> x * inv x == 1. Proof. auto with field. Qed.
 
     Lemma mul_cancel_r (x y z:F) : not (z == 0) -> x * z == y * z -> x == y.
     Proof.
       intros.
       assert (x * z * inv z == y * z * inv z) by
-          (match goal with [H: _ == _ |- _ ] => rewrite H; field end).
-      assert (x * z * inv z == x * (z * inv z)) by field.
-      assert (y * z * inv z == y * (z * inv z)) by field.
-      rewrite mul_inv_r, @ring_mul_1_r in * by assumption.
-      nsatz.
+          (match goal with [H: _ == _ |- _ ] => rewrite H; auto with field end).
+      assert (x * z * inv z == x * (z * inv z)) by auto with field.
+      assert (y * z * inv z == y * (z * inv z)) by auto with field.
+      rewrite mul_inv_r, @ring_mul_1_r in *; auto with field.
     Qed.
 
     Lemma mul_cancel_l (x y z:F) : not (z == 0) -> z * x == z * y -> x == y.
-    Proof. intros. eapply mul_cancel_r; eauto. nsatz. Qed.
+    Proof. intros. eauto using mul_cancel_r with field. Qed.
 
-    Lemma inv_unique (a:F) : forall x y, x * a == 1 -> y * a == 1 -> x == y.
-    Proof. nsatz. Qed.
+    Lemma inv_unique (a:F) : forall x y, x * a == 1 -> y * a == 1 -> x == y. Proof. auto with field. Qed.
     
     Lemma mul_nonzero_nonzero (a b:F) : not (a == 0) -> not (b == 0) -> not (a*b == 0).
-    Proof. intros. intro Hab. destruct (mul_zero_why _ _ Hab); intuition. Qed.
+    Proof. intros; intro Hab. destruct (mul_zero_why _ _ Hab); auto. Qed.
+    Hint Resolve mul_nonzero_nonzero : field_nonzero.
 
-    Lemma sub_diag_iff (x y:F) : x - y == 0 <-> x == y. Proof. split; nsatz. Qed.
+    Lemma inv_nonzero (x:F) : not(x == 0) -> not(inv x==0).
+    Proof.
+      intros Hx Hi.
+      assert (Hc:not (inv x*x==0)) by (rewrite field_inv_def; auto with field_nonzero); contradict Hc.
+      ring [Hi].
+    Qed.
+    Hint Resolve inv_nonzero : field_nonzero.
 
-    Lemma mul_same (x:F) : x*x == x^2%Z. reflexivity. Qed.
+    Lemma div_nonzero (x y:F) : not(x==0) -> not(y==0) -> not(x/y==0).
+    Proof.
+      unfold division, div_notation, div; auto with field_nonzero.
+    Qed.
+    Hint Resolve div_nonzero : field_nonzero.
+
+    Lemma pow_pos_nonzero (x:F) p : not(x==0) -> not(Ncring.pow_pos x p == 0).
+    Proof.
+      intros; induction p using Pos.peano_ind; try assumption; [].
+      rewrite Ncring.pow_pos_succ; eauto using mul_nonzero_nonzero.
+    Qed.
+    Hint Resolve pow_pos_nonzero : field_nonzero.
+
+    Lemma sub_diag_iff (x y:F) : x - y == 0 <-> x == y. Proof. auto with field. Qed.
+
+    Lemma mul_same (x:F) : x*x == x^2%Z. Proof. auto with field. Qed.
+
+    Lemma inv_mul (x y:F) : not(x==0) -> not (y==0) -> inv (x*y) == inv x * inv y.
+    Proof. intros;field;intuition. Qed.
+
+    Lemma pow_0_r (x:F) : x^0 == 1. Proof. reflexivity. Qed.
+
+    Lemma pow_succ_r (x:F) (n:Z) : not (x==0)\/(n>=0)%Z -> x^(n+1) == x * x^n.
+    Proof.
+      intros Hnz; unfold power, powZ, power_field, powZ; destruct n eqn:HSn.
+      - simpl; ring. 
+      - setoid_rewrite <-Pos2Z.inj_succ; rewrite Ncring.pow_pos_succ; ring.
+      - destruct (Z.succ (Z.neg p)) eqn:Hn.
+        + assert (p=1%positive) by (destruct p; simpl in *; try discriminate; auto).
+          subst; simpl in *; field. destruct Hnz; auto with field_nonzero.
+        + destruct p, p0; discriminate.
+        + setoid_rewrite Hn.
+          apply Z_neg_succ_neg in Hn; subst.
+          rewrite Ncring.pow_pos_succ; field;
+            destruct Hnz; auto with field_nonzero.
+    Qed.
+
+    Lemma pow_pred_r (x:F) (n:Z) : not (x==0) -> x^(n-1) == x^n/x.
+    Proof.
+      intros; unfold power, powZ, power_field, powZ; destruct n eqn:HSn.
+      - simpl. rewrite unfold_div; field.
+      - destruct (Z.pos p - 1) eqn:Hn.
+        + apply Z_pos_pred_0 in Hn; subst; simpl; field.
+        + apply Z_pos_pred_pos in Hn; subst.
+          rewrite Ncring.pow_pos_succ; field; auto with field_nonzero.
+        + destruct p; discriminate.
+      - rewrite Z_pred_neg, Ncring.pow_pos_succ; field; auto with field_nonzero.
+    Qed.
+          
+    Ltac pow_peano :=
+      repeat (setoid_rewrite pow_0_r 
+              || setoid_rewrite pow_succ_r
+              || setoid_rewrite pow_pred_r).
+    
+    Lemma pow_mul (x y:F) : forall (n:Z), not(x==0)/\not(y==0)\/(n>=0)%Z -> (x * y)^n == x^n * y^n.
+    Proof.
+      match goal with |- forall n, @?P n => eapply (Z.order_induction'_0 P) end.
+      { repeat intro. subst. reflexivity. }
+      - intros; cbv [power power_field powZ]; ring.
+      - intros n Hn IH Hxy.
+        repeat setoid_rewrite pow_succ_r; try rewrite IH; try ring; (right; omega).
+      - intros n Hn IH Hxy. destruct Hxy as [[]|?]; try omega; [].
+        repeat setoid_rewrite pow_pred_r; try rewrite IH; try field; auto with field_nonzero.
+    Qed.
+
+    Lemma pow_nonzero (x:F) : forall (n:Z), not(x==0) -> not(x^n==0).
+      match goal with |- forall n, @?P n => eapply (Z.order_induction'_0 P) end; intros; pow_peano;
+        auto with field_nonzero.
+      { repeat intro. subst. reflexivity. }
+    Qed.
+    Hint Resolve pow_nonzero : field_nonzero.
  
+    Lemma pow_inv (x:F) : forall (n:Z), not(x==0) -> inv x^n == inv (x^n).
+      match goal with |- forall n, @?P n => eapply (Z.order_induction'_0 P) end.
+      { repeat intro. subst. reflexivity. }
+      - intros; cbv [power power_field powZ]. field.
+      - intros n Hn IH Hx.
+        repeat setoid_rewrite pow_succ_r; try rewrite IH; try field; auto with field_nonzero.
+      - intros n Hn IH Hx. 
+        repeat setoid_rewrite pow_pred_r; try rewrite IH; try field; auto 3 with field_nonzero.
+    Qed.
+
+    Lemma pow_0_l : forall n, (n>0)%Z -> (0:F)^n==0.
+      match goal with |- forall n, @?P n => eapply (Z.order_induction'_0 P) end; intros; try omega.
+      { repeat intro. subst. reflexivity. }
+      setoid_rewrite pow_succ_r; [auto with field|right;omega].
+    Qed.
+
+    Lemma pow_div (x y:F) (n:Z) : not (y==0) -> not(x==0)\/(n >= 0)%Z -> (x/y)^n == x^n/y^n.
+    Proof.
+      intros Hy Hxn. unfold division, div_notation, div.
+      rewrite pow_mul, pow_inv; try field; destruct Hxn; auto with field_nonzero.
+    Qed.
+
+    Hint Extern 3 (_ >= _)%Z => omega : field_nonzero.
     Lemma issquare_mul (x y z:F) : not (y == 0) -> x^2%Z == z * y^2%Z -> (x/y)^2%Z == z.
-    Proof. intros. rewrite <-!mul_same; field_simplify_eq; nsatz. Qed.
+    Proof. intros. rewrite pow_div by (auto with field_nonzero); auto with field. Qed.
 
     Lemma issquare_mul_sub (x y z:F) : 0 == z*y^2%Z - x^2%Z -> (x/y)^2%Z == z \/ x == 0.
-    Proof.
-      destruct (eq_dec y 0); [right|left].
-      -
+    Proof. destruct (eq_dec y 0); [right|left]; auto using issquare_mul with field. Qed.
